# Chapter 4: The Schr√∂dinger Equation

<!-- ======================= -->
<!-- PROBLEM 4.1             -->
<!-- ======================= -->
## Problem 4.1

### Part a: "Pointwise ‚û° Weak"

Assume $\psi$ satisfies the free Shr√∂dinger equation pointwise:

$$
\frac{\partial \psi}{\partial t} - \frac{i\hbar}{2m} \frac{\partial^2 \psi}{\partial x^2} = 0. \tag{4.1.1}
$$

Take $\chi \in C_c^\infty(\mathbb{R}^2)$ a smooth compactly supported function and integrate

$$
0 = \int_{\mathbb{R}^2} dt\, dx\, \left( \frac{\partial \psi}{\partial t} - \frac{i\hbar}{2m} \frac{\partial^2 \psi}{\partial x^2} \right) \chi(t,x).
$$

Let's integrate by parts, first in $t$:

$$
\begin{align}
\int_{\mathbb{R}^2} dt\, dx\, \frac{\partial \psi}{\partial t} \chi(t,x) &= \int_{\mathbb{R}} dx\, \Bigl[ \psi(t,x)\chi(t,x) \Bigr]_{t=-\infty}^{t=+\infty} - \int_{\mathbb{R}^2} dt\, dx\, \psi(t,x) \frac{\partial \chi}{\partial t}(t,x) \\
&= - \int_{\mathbb{R}^2} dt\, dx\, \psi(t,x) \frac{\partial \chi}{\partial t}(t,x),
\end{align}
$$

where we used that $\chi$ is compactly supported, so it vanishes at $t = \pm \infty$.

The second term produces


$$
\begin{align}
\int_{\mathbb{R}^2} dt\, dx\, \frac{i\hbar}{2m} \frac{\partial^2 \psi}{\partial x^2} \chi(t,x) &= \frac{i\hbar}{2m} \int_{\mathbb{R}} dt\, \Bigl[ \frac{\partial \psi}{\partial x}(t,x) \chi(t,x) \Bigr]_{x=-\infty}^{x=+\infty} \\
& \quad- \frac{i\hbar}{2m} \int_{\mathbb{R}^2} dt\, dx\, \frac{\partial \psi}{\partial x}(t,x) \frac{\partial \chi}{\partial x}(t,x) \\
&=  \frac{i\hbar}{2m} \int_{\mathbb{R}^2} dt\, dx\, \psi(t,x) \frac{\partial^2 \chi}{\partial x^2}(t,x),
\end{align}
$$

so that Eqn. (4.1.1) becomes

$$
0 = \int_{\mathbb{R}^2} dt\, dx\, \psi(t,x) \left( -\frac{\partial \chi}{\partial t}(t,x) - \frac{i\hbar}{2m} \frac{\partial^2 \chi}{\partial x^2}(t,x) \right).
$$

That's the weak form of the Schr√∂dinger equation.

### Part a: "Weak ‚û° Pointwise"

Assume the weak form of the Schr√∂dinger equation holds:

$$
\int_{\mathbb{R}^2} dt\, dx\, \psi(t,x) \left(\frac{\partial \chi}{\partial t}(t,x) + \frac{i\hbar}{2m} \frac{\partial^2 \chi}{\partial x^2}(t,x) \right) = 0, \quad \forall \chi \in C_c^\infty(\mathbb{R}^2).
$$

Since $\psi$ is locally integrable we can repeat the same integration by parts as in part a, obtaining

$$
\int_{\mathbb{R}^2} dt\, dx\, \left( \frac{\partial \psi}{\partial t} - \frac{i\hbar}{2m} \frac{\partial^2 \psi}{\partial x^2} \right) \chi(t,x) = 0, \quad \forall \chi \in C_c^\infty(\mathbb{R}^2).
$$

Applying the result of Proposition A.23 we conclude that (with $f_2 = 0$)

$$
\frac{\partial \psi}{\partial t} - \frac{i\hbar}{2m} \frac{\partial^2 \psi}{\partial x^2} = 0
$$

### Part b

Fix $\chi \in C_c^\infty(\mathbb{R}^2)$, for each $t$, $\chi(\cdot, t) \in C_c^\infty(\mathbb{R})$ and so are $\partial_x \chi(\cdot, t)$ and $\partial_x^2 \chi(\cdot, t)$. Define

$$
S\chi(x, t) = \frac{\partial \chi}{\partial t}(x,t) + \frac{i\hbar}{2m} \frac{\partial^2 \chi}{\partial x^2}(x,t).
$$

For a fixed $t$

$$
\int_{\mathbb{R}} dx\, \psi(x,t) S\chi(x,t) = \frac{1}{2\pi}\int_{\mathbb{R}} dk\, \hat{\psi}(k, t) \widehat{S\chi}(-k,t), \tag{4.1.2}
$$

We need to calculate now $\widehat{S\chi}(k,t)$.

**Time derivative:**

$$
\frac{\partial \chi}{\partial t}(x,t) \xrightarrow{\mathcal{F}} \frac{\partial \hat{\chi}}{\partial t}(k,t).
$$

**Second spatial derivative:**

$$
\frac{\partial^2 \chi}{\partial x^2}(x,t) \xrightarrow{\mathcal{F}} -(ik)^2 \hat{\chi}(k,t) = -k^2 \hat{\chi}(k,t).
$$

Putting these together we have

$$
\widehat{S\chi}(k,t) = \frac{\partial \hat{\chi}}{\partial t}(k,t) - \frac{i\hbar}{2m} k^2 \hat{\chi}(k,t). \tag{4.1.3}
$$

Replacing Eqn. (4.1.3) into Eqn. (4.1.2) and integrating in time we obtain

$$
\begin{align}
\int_{\mathbb{R}^2} dt\, dx\, \psi(x,t) S\chi(x,t) &= \frac{1}{2\pi} \int_{\mathbb{R}^2} dt\,dk\, \hat{\psi}(k,t) \left( \frac{\partial }{\partial t}\hat{\chi}(-k,t) - \frac{i\hbar}{2m} k^2 \hat{\chi}(-k,t) \right) \\
&= -\frac{1}{2\pi} \int_{\mathbb{R}^2} dt\,dk\, \left( \frac{\partial}{\partial t}\hat{\psi}(k,t) + \frac{i\hbar}{2m} k^2 \hat{\psi}(k,t) \right) \hat{\chi}(-k,t) \\
&= -\frac{1}{2\pi} \int_{\mathbb{R}^2} dt\,dk\, \left( -\frac{i\hbar k^2}{2m}\hat{\psi}(k, t) + \frac{i\hbar}{2m} k^2 \hat{\psi}(k,t) \right) \hat{\chi}(-k,t) \\
&= 0
\end{align}
$$

That is, $\psi$ satisfies the weak form of the Schr√∂dinger equation.

<!-- ======================= -->
<!-- PROBLEM 4.2             -->
<!-- ======================= -->
## Problem 4.2 üå∂Ô∏è


### Part a

To prove

$$
\left(\int_{-\infty}^\infty dx\, e^{-x^2/2a} \right)^2 = \int_{-\infty}^\infty \int_{-\infty}^\infty dx\, dy\, e^{-(x^2 + y^2)/2a},
$$

first we need to show that RHS converges,

$$
\int_{-\infty}^\infty \int_{-\infty}^\infty dx\, dy\, |e^{-(x^2 + y^2)/2a}| = \int_{-\infty}^\infty \int_{-\infty}^\infty dx\, dy\, e^{-(x^2 + y^2)\Re(1/2a)}.
$$

Let's consider three cases:

**1. $\Re(a) < 0$**

In that case the exponential blows up and the integral diverges.

**2. $\Re(a) = 0$**

The modulus is constant, so the integral does not converge absolutely. Fubini's theorem does not apply directly; this case requires a separate argument (see [Part c](#part-c)).

**3. $\Re(a) > 0$**

Call

$$
\gamma = \Re\left(\frac{1}{2a}\right) > 0,
$$

then

$$
\int_{-\infty}^\infty \int_{-\infty}^\infty dx\, dy\, e^{-(x^2 + y^2)\Re(1/2a)} = \int_{-\infty}^\infty \int_{-\infty}^\infty dx\, dy\, e^{-\gamma (x^2 + y^2)}.
$$

This integral converges since $\gamma > 0$, equivalently $\Re(a) > 0$, since

$$
\Re\left(\frac{1}{2a}\right) = \frac{\Re(a)}{2|a|^2}.
$$

We then have

$$
\int_{-\infty}^\infty \int_{-\infty}^\infty dx\, dy\, |e^{-(x^2 + y^2)/2a}| < \infty,
$$

which allows us to use Fubini's theorem to write

$$
\begin{align}
\int_{-\infty}^\infty \int_{-\infty}^\infty dx\, dy\, e^{-(x^2 + y^2)/2a} &= \int_{-\infty}^\infty dx\, e^{-x^2/2a} \left(\int_{-\infty}^\infty dy\, e^{-y^2/2a} \right) \\
&= \left(\int_{-\infty}^\infty dx\, e^{-x^2/2a} \right)^2.
\end{align}
$$

Now we can calculate the integral for the $\Re(a) > 0$ case. Using polar coordinates $x = r\cos\theta$, $y = r\sin\theta$, $dx\, dy = r\, dr\, d\theta$ we have

$$
\begin{align}
\int_{-\infty}^\infty \int_{-\infty}^\infty dx\, dy\, e^{-(x^2 + y^2)/2a} &= \int_0^{2\pi} d\theta \int_0^\infty dr\, r\, e^{-r^2/2a} \\
&= 2\pi \int_0^\infty dr\, r\, e^{-r^2/2a} \\
&= 2\pi \left[-a e^{-r^2/2a} \right]_{r=0}^{r=\infty} \\
&= 2\pi a.
\end{align}
$$

Thus

$$
\int_{-\infty}^\infty dx\, e^{-x^2/2a} = \sqrt{2\pi a}, \quad \Re(a) > 0.
$$

### Part b


$$
\begin{align}
\frac{d}{dx}\left(\frac{a}{x}e^{-x^2/2a}\right) &= -\frac{a}{x^2}e^{-x^2/2a} + \frac{a}{x} \left(-\frac{x}{a}\right) e^{-x^2/2a} \\
&= -\frac{a}{x^2}e^{-x^2/2a} - e^{-x^2/2a}.
\end{align}
$$

Thus

$$
\int_A^B dx\, e^{-x^2/2a} = -\left.\frac{a}{x} e^{-x^2/2a} \right|_{A}^{B} - \int_A^B dx\, \frac{a}{x^2}e^{-x^2/2a}.
$$

!!! warning "Typo in book"
    There is a typo in the book's version of this equation: the second term on the right-hand side is missing a minus sign.


!!! question "$x=0$?"
    I've been going around in circles about the statement $A, B > 0$ in the problem, I think it should be $0 < A < B$ to avoid the singularity at $x=0$, which was introduced when integrating by parts, the factors $a/x$ and $a/x^2$ are not defined at $x=0$, which would make the equation invalid.

    I will come back to this later.

### Part c

**Step 1: Uniform bound on the tail integral.**

Let $a = \alpha + i\beta$ with $\beta \neq 0$ fixed and $\alpha \in [0, 1]$. From Part b, we have the identity

$$
\int_A^\infty dx\, e^{-x^2/2a} = -\left.\frac{a}{x} e^{-x^2/2a} \right|_{A}^{\infty} - \int_A^\infty dx\, \frac{a}{x^2}e^{-x^2/2a}.
$$

Consider each term separately.

**For the boundary term**

Note that

$$
|a| = |\alpha + i\beta| = \sqrt{\alpha^2 + \beta^2}  \leq \sqrt{1 + \beta^2},
$$

therefore

$$
\left|\frac{a}{x} e^{-x^2/2a}\right| = \frac{|a|}{x} e^{-x^2 \Re(1/2a)} = \frac{|a|}{x} e^{-x^2 \alpha/(2|a|^2)} \leq \frac{\sqrt{1 + \beta^2}}{x} \to 0.
$$

At $x = A$:

$$
\left|\frac{a}{A} e^{-A^2/2a}\right| \leq \frac{\sqrt{1 + \beta^2}}{A}.
$$

**For the integral term**

$$
\left|\int_A^\infty dx\, \frac{a}{x^2} e^{-x^2/2a}\right| \leq |a| \int_A^\infty dx\, \frac{1}{x^2} e^{-x^2 \alpha/(2|a|^2)} \leq |a| \int_A^\infty dx\, \frac{1}{x^2} = \frac{|a|}{A}.
$$

Combining these estimates:

$$
\left|\int_A^\infty dx\, e^{-x^2/2a}\right| \leq \frac{2|a|}{A} \leq \frac{2\sqrt{1 + \beta^2}}{A}.
$$

This bound is uniform in $\alpha \in [0, 1]$ and vanishes as $A \to \infty$.

**Step 2: Extension to $\Re(a) = 0$.**

For $\alpha > 0$, we have established that

$$
\int_{-\infty}^\infty dx\, e^{-x^2/2a} = \sqrt{2\pi a}.
$$

By symmetry of the integrand, this equals $2\int_0^\infty dx\, e^{-x^2/2a}$.

Fix $\beta \neq 0$ and define $f(\alpha) = \int_0^\infty dx\, e^{-x^2/2(\alpha + i\beta)}$ for $\alpha \in [0, 1]$. Split the integral:

$$
f(\alpha) = \int_0^A dx\, e^{-x^2/2(\alpha + i\beta)} + \int_A^\infty dx\, e^{-x^2/2(\alpha + i\beta)}.
$$

The first integral is a continuous function of $\alpha$ (the integrand is continuous and bounded on $[0, A] \times [0, 1]$). By Step 1, the second integral is bounded by $2\sqrt{1+\beta^2}/A$ uniformly in $\alpha$, for each $\varepsilon > 0$, we can then choose $A$ large enough so that the second integral is smaller than $\varepsilon/2$, thus

$$
|f(\alpha) - f(0)| \leq \left|\int_0^A dx\, \left(e^{-x^2/2(\alpha + i\beta)} - e^{-x^2/2(i\beta)}\right)\right| + \varepsilon.
$$

As $\alpha \to 0^+$, the first term vanishes by continuity. Thus $f$ is continuous at $\alpha = 0$, and

$$
\int_0^\infty dx\, e^{-x^2/2(i\beta)} = \lim_{\alpha \to 0^+} \int_0^\infty dx\, e^{-x^2/2(\alpha + i\beta)} = \lim_{\alpha \to 0^+} \frac{1}{2}\sqrt{2\pi(\alpha + i\beta)} = \frac{1}{2}\sqrt{2\pi i\beta}.
$$

Therefore, for $a = i\beta$ with $\beta \neq 0$:

$$
\int_{-\infty}^\infty dx\, e^{-x^2/2a} = \sqrt{2\pi a}.
$$

The formula extends to all $a$ with $\Re(a) \geq 0$ and $a \neq 0$.

### Part d

$$
\begin{align}
\frac{1}{2\pi}\int_{-\infty}^\infty dk\, e^{ikx} e^{-i\hbar k^2 t/2m} &= \frac{1}{2\pi} \int_{-\infty}^\infty dk\, \exp\left({- \frac{i\hbar t}{2m} \left( k^2 - \frac{2m x}{\hbar t} k \right)}\right) \\
&= \frac{1}{2\pi} \int_{-\infty}^\infty dk\, \exp\left({- \frac{i\hbar t}{2m} \left( k - \frac{m x}{\hbar t} \right)^2 + \frac{i m x^2}{2\hbar t}}\right) \\
&= \frac{1}{2\pi} e^{i m x^2/2\hbar t} \int_{-\infty}^\infty dk\, \exp\left(- \frac{i\hbar t}{2m} \left( k - \frac{m x}{\hbar t} \right)^2 \right) \\
&= \frac{1}{2\pi} e^{i m x^2/2\hbar t} \int_{-\infty}^\infty dk'\, e^{- i\hbar t k'^2/2m } \\
&= \frac{1}{2\pi} e^{i m x^2/2\hbar t} \sqrt{2\pi \frac{2m}{i\hbar t}} \\
&= \sqrt{\frac{m}{2\pi i \hbar t}} e^{i m x^2/2\hbar t}.
\end{align}
$$

<!-- ======================= -->
<!-- PROBLEM 4.3             -->
<!-- ======================= -->
## Problem 4.3

We need to prove three things

### Well-definedness

Since Shcwartz functions are in $L^2(\mathbb{R})$, then

$$
|(\phi * \psi)(x)| \leq \int_{-\infty}^\infty dy\, |\phi(x - y)| |\psi(y)| \leq \|\phi\|_2 \|\psi\|_2 < \infty,
$$


### Differentiability

Consider

$$
\frac{(\phi * \psi)(x + h) - (\phi * \psi)(x)}{h} = \int_{-\infty}^\infty dy\, \frac{\phi(x + h - y) - \phi(x - y)}{h} \psi(y).
$$

By the mean value theorem, for each $y$ there exists $\xi_h \in (x - y, x + h - y)$ such that

$$
\frac{\phi(x + h - y) - \phi(x - y)}{h} = \phi'(\xi_h).
$$

Since $\phi \in \mathcal{S}(\mathbb{R})$, its derivative $\phi' \in \mathcal{S}(\mathbb{R})$ as well. In particular, $\phi'$ is bounded: $|\phi'(z)| \leq M$ for all $z \in \mathbb{R}$.

Thus the integrand is bounded by

$$
\left|\frac{\phi(x + h - y) - \phi(x - y)}{h} \psi(y)\right| \leq M |\psi(y)|,
$$

which is integrable since $\psi \in L^2(\mathbb{R})$. More precisely, we use that $\phi' \in L^2$ to get

$$
\int_{-\infty}^\infty dy\, |\phi'(x - y)| |\psi(y)| \leq \|\phi'\|_2 \|\psi\|_2 < \infty.
$$

By the dominated convergence theorem, we can pass the limit inside the integral:

$$
\begin{align}
(\phi * \psi)'(x) &= \lim_{h \to 0} \int_{-\infty}^\infty dy\, \frac{\phi(x + h - y) - \phi(x - y)}{h} \psi(y) \\
&= \int_{-\infty}^\infty dy\, \phi'(x - y) \psi(y) = (\phi' * \psi)(x).
\end{align}
$$

!!! warning "$L_2$ vs $L_1$"
    The statement "bounded by $M|\psi(y)|$, which is integrable" may be wrong. I am not convinced that being in $L^2$ implies being in $L^1$. Come back to this later.

### Smoothness

Since $\phi \in \mathcal{S}(\mathbb{R})$, all derivatives $\phi^{(n)} \in \mathcal{S}(\mathbb{R})$. By induction, applying the [Differentiability](#differentiability) argument repeatedly leads to

$$
(\phi * \psi)^{(n)} = \phi^{(n)} * \psi.
$$

Each $\phi^{(n)}$ is Schwartz, hence in $L^2$, so the same argument shows each derivative exists and is continuous.

Therefore $\phi * \psi \in C^\infty(\mathbb{R})$.

<!-- ======================= -->
<!-- PROBLEM 4.4             -->
<!-- ======================= -->
## Problem 4.4

### Part a
Define

$$
\hat{\psi}(k, t) = \int_{\mathbb{R}} dx\, e^{-ikx} \psi(x, t).
$$

Since $\psi(\cdot, t)$ is a "nice" function we can differentiate under the integral sign and any boundary terms vanish. Thus

$$
\begin{align}
\frac{\partial \hat{\psi}}{\partial t}(k, t) &= \int_{\mathbb{R}} dx\, e^{-ikx} \frac{\partial \psi}{\partial t}(x, t) \\
&= \alpha \int_{\mathbb{R}} dx\, e^{-ikx} \frac{\partial^2 \psi}{\partial x^2}(x, t) \\
&= \alpha \left[ e^{-ikx} \frac{\partial \psi}{\partial x}(x, t) \right]_{x=-\infty}^{x=+\infty} - \alpha \int_{\mathbb{R}} dx\, \frac{\partial}{\partial x} \left( e^{-ikx} \right) \frac{\partial \psi}{\partial x}(x, t) \\
&= i\alpha k \int_{\mathbb{R}} dx\, e^{-ikx} \frac{\partial \psi}{\partial x}(x, t) \\
&= i\alpha k \left[ e^{-ikx} \psi(x, t) \right]_{x=-\infty}^{x=+\infty} - i\alpha k \int_{\mathbb{R}} dx\, \frac{\partial}{\partial x} \left( e^{-ikx} \right) \psi(x, t) \\
&= -\alpha k^2 \int_{\mathbb{R}} dx\, e^{-ikx} \psi(x, t) \\
&= -\alpha k^2 \hat{\psi}(k, t).
\end{align}
$$

This is a first-order ODE in $t$ for each fixed $k$, with solution

$$
\hat{\psi}(k, t) = \hat{\psi}(k, 0) e^{-\alpha k^2 t} = \hat{\psi}_0(k) e^{-\alpha k^2 t}.
$$

### Part b

Taking the Fourier inverse

$$
\begin{align}
\psi(x,t) &= \frac{1}{2\pi} \int_{\mathbb{R}} dk\, e^{ikx} \hat{\psi}(k,t) = \frac{1}{2\pi} \int_{\mathbb{R}} dk\, e^{ikx} \hat{\psi}_0(k) e^{-\alpha k^2 t} \\
&= \frac{1}{2\pi} \int_{\mathbb{R}} dk\, e^{ikx} \hat{G}(k, t) \hat{\psi}_0(k) \\
&= \mathcal{F}^{-1}[\hat{G}(\cdot, t) \hat{\psi}_0](x),
\end{align}
$$

Where $\hat{G}(k, t) = e^{-\alpha k^2 t}$ is the Fourier transform of the heat kernel $G(x, t)$

$$
\begin{align}
G(x, t) &= \frac{1}{2\pi} \int_{\mathbb{R}} dk\, e^{ikx} e^{-\alpha k^2 t} \\
&= \frac{1}{2\pi} \int_{\mathbb{R}} dk\, \exp\left(-\alpha t \left( k^2 - \frac{ikx}{\alpha t} \right) \right) \\
&= \frac{1}{2\pi} \int_{\mathbb{R}} dk\, \exp\left(-\alpha t \left( k - \frac{ix}{2\alpha t} \right)^2 - \frac{x^2}{4\alpha t} \right) \\
&= \frac{1}{2\pi} e^{-x^2/4\alpha t} \int_{\mathbb{R}} dk\, e^{-\alpha t (k - ix/2\alpha t)^2} \\
&= \frac{1}{2\pi} e^{-x^2/4\alpha t} \sqrt{\frac{\pi}{\alpha t}} \\
&= \frac{1}{\sqrt{4\pi \alpha t}} e^{-x^2/4\alpha t}. \qquad t > 0
\end{align}
$$

<!-- ======================= -->
<!-- PROBLEM 4.5             -->
<!-- ======================= -->
## Problem 4.5

$$
Q(x) = \frac{1}{(\theta_0')^2}\left(\frac{1}{A_0} \frac{d^2 A_0}{dx^2}\right) = \left(\frac{\hbar}{Lp_0}\right)^2\left( \frac{(x - x_0)^2}{L^2} - 1 \right).
$$

Define $\epsilon = \hbar / (L p_0)$, and consider a region where the amplitude is not exponentially small, i.e., $|x - x_0| \leq C L$, for some $C = O(1)$. In that region

$$
Q(x) \leq \epsilon^2 (C^2 - 1) = O(\epsilon^2) \ll 1.
$$

That is, in the "bulk" of the wavepacket, the quantity $Q(x)$ is small.

Assume now that $Q(x) \sim 1$, then

$$
\epsilon^2 \left( \frac{(x - x_0)^2}{L^2} - 1 \right) \sim 1.
$$

Or equivalently

$$
\frac{(x - x_0)^2}{L^2} - 1 \sim \frac{1}{\epsilon^2} \implies |x - x_0| \sim L \sqrt{1 + \frac{1}{\epsilon^2}} \sim \frac{L}{\epsilon} = \frac{\hbar}{p_0}.
$$

In that region

$$
A_0(x) \sim \exp\left(-\frac{1}{2\epsilon^2}\right) \ll 1,
$$

which is exponentially small for small $\epsilon$. We thus have

- In the bulk of the wavepacket, $Q(x) \ll 1$.
- $Q(x) \sim 1$ only in the tails of the wavepacket, where the amplitude is exponentially small.

<!-- ======================= -->
<!-- PROBLEM 4.6             -->
<!-- ======================= -->
## Problem 4.6


### Part a
For a free particle $\psi(x) = \psi_0 \exp(i(kx - \omega(k)t))$ we get from the Klein-Gordon equation

$$
\left(\frac{1}{c^2}(-\omega(k)^2) - (-k^2) + \frac{m^2 c^2}{\hbar^2}\right) \psi(x) = 0,
$$

Or equivalently

$$
\omega(k)^2 = c^2 k^2 + \frac{m^2 c^4}{\hbar^2}.
$$

Using $E = \hbar \omega$ and $p = \hbar k$ we get the relativistic energy-momentum relation

$$
E^2 = p^2 c^2 + m^2 c^4.
$$

### Part b

Clearly

$$
v_{\mathrm{phase}} = \frac{\omega(k)}{k} = \frac{c}{k} \sqrt{k^2 + \frac{m^2 c^2}{\hbar^2}} = c \sqrt{1 + \frac{m^2 c^2}{\hbar^2 k^2}} > c.
$$

And

$$
v_{\mathrm{group}} = \frac{d\omega}{dk} = \frac{c^2 k}{\sqrt{k^2 + m^2 c^2/\hbar^2}} < c.
$$

Also

$$
v_{\mathrm{phase}} \cdot v_{\mathrm{group}} = \frac{c\sqrt{k^2 + m^2c^2/\hbar^2}}{k} \cdot \frac{c^2 k}{\sqrt{k^2 + m^2c^2/\hbar^2}} = c^2
$$


<!-- ======================= -->
<!-- PROBLEM 4.7             -->
<!-- ======================= -->
## Problem 4.7


For a free particle with $H = P^2/2m$, Ehrenfest's theorem gives

$$
\frac{d\langle X \rangle}{dt} = \frac{i}{\hbar}\langle [H, X] \rangle = \frac{\langle P \rangle}{m}.
$$

And

$$
\begin{align}
\frac{d\langle X^2 \rangle}{dt} &= \frac{i}{\hbar} \langle[H, X^2]\rangle = \frac{i}{\hbar} \left\langle \left[\frac{P^2}{2m}, X^2\right] \right\rangle \\
&= \frac{i}{2m\hbar} \langle P[P, X^2] + [P, X^2]P \rangle = \frac{i}{2m\hbar} \langle P(-2i\hbar X) + (-2i\hbar X)P \rangle \\
&= \frac{1}{m} \langle PX + XP \rangle.
\end{align}
$$

Now, since $(\Delta_\psi X)^2 = \langle X^2 \rangle - \langle X \rangle^2$:

$$
\frac{d(\Delta_\psi X)^2}{dt} = \frac{d\langle X^2 \rangle}{dt} - 2\langle X \rangle \frac{d\langle X \rangle}{dt} = \frac{1}{m}\left(\langle PX + XP \rangle - 2\langle X \rangle \langle P \rangle\right).
$$

Define centered operators $\tilde{X} = X - \langle X \rangle$ and $\tilde{P} = P - \langle P \rangle$. Then

$$
\langle PX + XP \rangle - 2\langle X \rangle \langle P \rangle = \langle \tilde{P}\tilde{X} + \tilde{X}\tilde{P} \rangle.
$$

Therefore

$$
\frac{d(\Delta_\psi X)}{dt}  = \frac{1}{2\Delta_\psi X} \frac{d(\Delta_\psi X)^2}{dt} = \frac{\langle \tilde{P}\tilde{X} + \tilde{X}\tilde{P} \rangle}{2m \Delta_\psi X}. \tag{4.7.1}
$$


For self-adjoint operators, the Cauchy-Schwarz inequality gives

$$
|\langle \tilde{P}\tilde{X} \rangle| \leq \langle \tilde{P}^2 \rangle^{1/2}\langle \tilde{X}^2 \rangle^{1/2} = \Delta_\psi P \cdot \Delta_\psi X.
$$

Similarly $|\langle \tilde{X}\tilde{P} \rangle| \leq \Delta_\psi X \cdot \Delta_\psi P$. Therefore

$$
|\langle \tilde{P}\tilde{X} + \tilde{X}\tilde{P} \rangle| \leq 2 \Delta_\psi X \cdot \Delta_\psi P.
$$

Plugging this into Eqn. (4.7.1) we obtain

$$
\left|\frac{d(\Delta_\psi X)}{dt}\right| = \frac{|\langle \tilde{P}\tilde{X} + \tilde{X}\tilde{P} \rangle|}{2m \Delta_\psi X} \leq \frac{2 \Delta_\psi X \cdot \Delta_\psi P}{2m \Delta_\psi X} = \frac{\Delta_\psi P}{m}.
